refine actions, and provide heap extension as an action with pre & postconditions on freshness

pulse/lib/pulse/core/PulseCore.Heap.fsti
@@ -405,8 +405,14 @@ val weaken_free_above (h:heap) (a b:nat)
   The base type for an action is indexed by two separation logic propositions, representing
   the heap specification of the action before and after.
 *)
-let pre_action (fp:slprop u#a) (a:Type u#b) (fp':a -> slprop u#a) =
-  full_hheap fp -> (x:a & full_hheap (fp' x))
+let trivial_pre (h:full_heap) : prop = True
+module T = FStar.Tactics
+let pre_action (#[T.exact (`trivial_pre)]pre:full_heap -> prop)
+               (#[T.exact (`trivial_pre)]post:full_heap -> prop)
+               (fp:slprop u#a)
+               (a:Type u#b)
+               (fp':a -> slprop u#a)
+  = h0:full_hheap fp { pre h0 } -> res:(x:a & full_hheap (fp' x)) { post (dsnd res) }
 
 (**
   This is how the heaps before and after the action relate:
@@ -414,11 +420,18 @@ let pre_action (fp:slprop u#a) (a:Type u#b) (fp':a -> slprop u#a) =
   - not allocating any new references;
   - preserving the validity of any heap proposition affecting any frame
 *)
+let immut_heap = true
+let mut_heap = false
+let allocs = true
+let no_allocs = false
 unfold
-let action_related_heaps (frame:slprop) (h0 h1:full_heap) =
+let action_related_heaps 
+      (#[T.exact (`mut_heap)] immut:bool)
+      (#[T.exact (`no_allocs)] allocates:bool)
+      (h0 h1:full_heap) =
   heap_evolves h0 h1 /\
-  (forall ctr. h0 `free_above_addr` ctr ==> h1 `free_above_addr` ctr) /\
-  (forall (hp:hprop frame). hp h0 == hp h1)
+  (not allocates ==> (forall ctr. h0 `free_above_addr` ctr ==> h1 `free_above_addr` ctr)) /\
+  (immut ==> h0 == h1)
 
 (**
   We only want to consider heap updates that are "frame-preserving", meaning that they only
@@ -429,19 +442,26 @@ let action_related_heaps (frame:slprop) (h0 h1:full_heap) =
 *)
 let is_frame_preserving
   (#a: Type u#a)
+  (#pre #post:_)
   (#fp: slprop u#b)
   (#fp': a -> slprop u#b)
-  (f:pre_action fp a fp')
+  (immut:bool)
+  (allocates:bool)
+  (f:pre_action #pre #post fp a fp')
   =
-  forall (frame: slprop u#b) (h0:full_hheap (fp `star` frame)).
+  forall (frame: slprop u#b) (h0:full_hheap (fp `star` frame) { pre h0 }).
      (affine_star fp frame h0;
       let (| x, h1 |) = f h0 in
       interp (fp' x `star` frame) h1 /\
-      action_related_heaps frame h0 h1)
+      action_related_heaps #immut #allocates h0 h1)
 
 (** Every action is frame-preserving *)
-let action (fp:slprop u#b) (a:Type u#a) (fp':a -> slprop u#b) =
-  f:pre_action fp a fp'{ is_frame_preserving f }
+let action (#[T.exact (`mut_heap)] immut:bool)
+           (#[T.exact (`no_allocs)] allocates:bool)
+           (#[T.exact (`trivial_pre)]pre:full_heap -> prop)
+           (#[T.exact (`trivial_pre)]post:full_heap -> prop)
+           (fp:slprop u#b) (a:Type u#a) (fp':a -> slprop u#b) =
+  f:pre_action #pre #post fp a fp'{ is_frame_preserving immut allocates f }
 
 (**
   We define a second, but equivalent, type for actions that
@@ -458,18 +478,16 @@ let action_with_frame
     h0:full_hheap (fp `star` frame) ->
     Pure (x:a & full_hheap (fp' x `star` frame))
       (requires True)
-      (ensures fun (| x, h1 |) -> action_related_heaps frame h0 h1)
+      (ensures fun (| x, h1 |) -> action_related_heaps #immut_heap #no_allocs h0 h1)
 
 (**
   Two heaps [h0] and [h1] are frame-related if you can get from [h0] to [h1] with a
   frame-preserving update.
 *)
-let frame_related_heaps (h0 h1:full_heap) (fp0 fp1 frame:slprop) (allocates:bool) =
+let frame_related_heaps (h0 h1:full_heap) (fp0 fp1 frame:slprop) (immut:bool) (allocates:bool) =
   interp (fp0 `star` frame) h0 ==>
   interp (fp1 `star` frame) h1 /\
-  heap_evolves h0 h1 /\
-  (forall (hp:hprop frame). hp h0 == hp h1) /\
-  (not allocates ==> (forall ctr. h0 `free_above_addr` ctr ==> h1 `free_above_addr` ctr))
+  action_related_heaps #immut #allocates h0 h1
 
 
 (**
@@ -478,14 +496,15 @@ let frame_related_heaps (h0 h1:full_heap) (fp0 fp1 frame:slprop) (allocates:bool
 *)
 let action_framing
   (#a: Type u#a)
+  (#immut #allocates:bool)
   (#fp: slprop u#b)
   (#fp': a -> slprop u#b)
-  ($f:action fp a fp')
+  ($f:action #immut #allocates fp a fp')
   (frame:slprop) (h0:full_hheap (fp `star` frame))
     : Lemma (
       affine_star fp frame h0;
       let (| x, h1 |) = f h0 in
-      frame_related_heaps h0 h1 fp (fp' x) frame false
+      frame_related_heaps h0 h1 fp (fp' x) frame immut allocates
     )
   =
   affine_star fp frame h0;
@@ -527,7 +546,8 @@ val sel_action
   (#pcm:pcm a)
   (r:ref a pcm)
   (v0:erased a)
-    : action (pts_to r v0) (v:a{compatible pcm v0 v}) (fun _ -> pts_to r v0)
+    : action #immut_heap #no_allocs
+       (pts_to r v0) (v:a{compatible pcm v0 v}) (fun _ -> pts_to r v0)
 
 (**
   A version of select that incorporates a ghost update of local
@@ -539,7 +559,7 @@ val select_refine (#a:_) (#p:_)
                   (f:(v:a{compatible p x v}
                       -> GTot (y:a{compatible p y v /\
                                   FStar.PCM.frame_compatible p x v y})))
-   : action (pts_to r x)
+   : action #immut_heap #no_allocs (pts_to r x)
             (v:a{compatible p x v /\ p.refine v})
             (fun v -> pts_to r (f v))
 
@@ -547,7 +567,7 @@ val select_refine (#a:_) (#p:_)
 (** Updating a ref cell for a user-defined PCM *)
 val upd_gen_action (#a:Type) (#p:pcm a) (r:ref a p) (x y:Ghost.erased a)
                    (f:FStar.PCM.frame_preserving_upd p x y)
-  : action (pts_to r x)
+  : action #mut_heap #no_allocs (pts_to r x)
            unit
            (fun _ -> pts_to r y)
 
@@ -561,7 +581,7 @@ val upd_action
   (r:ref a pcm)
   (v0:FStar.Ghost.erased a)
   (v1:a {FStar.PCM.frame_preserving pcm v0 v1 /\ pcm.refine v1})
-  : action (pts_to r v0) unit (fun _ -> pts_to r v1)
+  : action #mut_heap #no_allocs (pts_to r v0) unit (fun _ -> pts_to r v1)
 
 (** Deallocating a reference, by actually replacing its value by the unit of the PCM *)
 val free_action
@@ -569,7 +589,7 @@ val free_action
   (#pcm:pcm a)
   (r:ref a pcm)
   (v0:FStar.Ghost.erased a {exclusive pcm v0 /\ pcm.refine pcm.FStar.PCM.p.one})
-  : action (pts_to r v0) unit (fun _ -> pts_to r pcm.FStar.PCM.p.one)
+  : action #mut_heap #no_allocs (pts_to r v0) unit (fun _ -> pts_to r pcm.FStar.PCM.p.one)
 
 
 (** Splitting a permission on a composite resource into two separate permissions *)
@@ -579,7 +599,7 @@ val split_action
   (r:ref a pcm)
   (v0:FStar.Ghost.erased a)
   (v1:FStar.Ghost.erased a{composable pcm v0 v1})
-  : action (pts_to r (v0 `op pcm` v1)) unit (fun _ -> pts_to r v0 `star` pts_to r v1)
+  : action #immut_heap #no_allocs (pts_to r (v0 `op pcm` v1)) unit (fun _ -> pts_to r v0 `star` pts_to r v1)
 
 (** Combining separate permissions into a single composite permission *)
 val gather_action
@@ -588,14 +608,15 @@ val gather_action
   (r:ref a pcm)
   (v0:FStar.Ghost.erased a)
   (v1:FStar.Ghost.erased a)
-  : action (pts_to r v0 `star` pts_to r v1) (_:unit{composable pcm v0 v1}) (fun _ -> pts_to r (op pcm v0 v1))
+  : action #immut_heap #no_allocs
+    (pts_to r v0 `star` pts_to r v1) (_:unit{composable pcm v0 v1}) (fun _ -> pts_to r (op pcm v0 v1))
 
 val pts_to_not_null_action 
       (#a:Type u#a)
       (#pcm:pcm a)
       (r:erased (ref a pcm))
       (v:Ghost.erased a)
-: action 
+: action #immut_heap #no_allocs
     (pts_to r v)
     (squash (not (is_null r)))
     (fun _ -> pts_to r v)
@@ -606,53 +627,51 @@ val extend
   (#pcm:pcm a)
   (x:a{compatible pcm x x /\ pcm.refine x})
   (addr:nat)
-  (h:full_heap{h `free_above_addr` addr})
-  : (
-    r:ref a pcm
-    & h':full_heap{
-      (forall (frame: slprop u#a).
-        frame_related_heaps h h' emp (pts_to r x) frame (true)) /\
-        h' `free_above_addr` (addr + 1) /\
-        heap_evolves h h'
-    }
-  )
+  : action
+      #mut_heap #allocs
+      #(fun h -> h `free_above_addr` addr)
+      #(fun h -> h `free_above_addr` (addr + 1))      
+      emp 
+      (ref a pcm)
+      (fun r -> pts_to r x)
 
 val frame (#a:Type)
+          #immut #allocates #hpre #hpost
           (#pre:slprop)
           (#post:a -> slprop)
           (frame:slprop)
-          ($f:action pre a post)
-  : action (pre `star` frame) a (fun x -> post x `star` frame)
+          ($f:action #immut #allocates #hpre #hpost pre a post)
+  : action #immut #allocates #hpre #hpost (pre `star` frame) a (fun x -> post x `star` frame)
 
 val change_slprop (p q:slprop)
                   (proof: (h:heap -> Lemma (requires interp p h) (ensures interp q h)))
-  : action p unit (fun _ -> q)
+  : action #immut_heap #no_allocs p unit (fun _ -> q)
 
-module U = FStar.Universe
+// module U = FStar.Universe
 
-val id_elim_star (p q:slprop) (h:heap)
-  : Pure (erased heap & erased heap )
-         (requires (interp (p `star` q) h))
-         (ensures (fun (hl, hr) -> disjoint hl hr
-                              /\ h == join hl hr
-                              /\ interp p hl
-                              /\ interp q hr))
+// val id_elim_star (p q:slprop) (h:heap)
+//   : Pure (erased heap & erased heap )
+//          (requires (interp (p `star` q) h))
+//          (ensures (fun (hl, hr) -> disjoint hl hr
+//                               /\ h == join hl hr
+//                               /\ interp p hl
+//                               /\ interp q hr))
 
-val id_elim_exists (#a:Type) (p : a -> slprop) (h:heap)
-  : Pure (erased a)
-         (requires (interp (h_exists p) h))
-         (ensures (fun x -> interp (p x) h))
+// val id_elim_exists (#a:Type) (p : a -> slprop) (h:heap)
+//   : Pure (erased a)
+//          (requires (interp (h_exists p) h))
+//          (ensures (fun x -> interp (p x) h))
 
 
-let is_frame_monotonic #a (p : a -> slprop) : prop =
-  forall x y m frame. interp (p x `star` frame) m /\ interp (p y) m ==> interp (p y `star` frame) m
+// let is_frame_monotonic #a (p : a -> slprop) : prop =
+//   forall x y m frame. interp (p x `star` frame) m /\ interp (p y) m ==> interp (p y `star` frame) m
 
-let is_witness_invariant #a (p : a -> slprop) =
-  forall x y m. interp (p x) m /\ interp (p y) m ==> x == y
+// let is_witness_invariant #a (p : a -> slprop) =
+//   forall x y m. interp (p x) m /\ interp (p y) m ==> x == y
 
-val witinv_framon (#a:_) (p : a -> slprop)
-  : Lemma (requires (is_witness_invariant p))
-          (ensures (is_frame_monotonic p))
+// val witinv_framon (#a:_) (p : a -> slprop)
+//   : Lemma (requires (is_witness_invariant p))
+//           (ensures (is_frame_monotonic p))
 
 
 (**
@@ -668,18 +687,18 @@ val intro_exists (#a:_) (p:a -> slprop) (x:erased a)
   : action_with_frame (p x) unit (fun _ -> h_exists p)
   
 val lift_h_exists (#a:_) (p:a -> slprop)
-  : action (h_exists p) unit
-           (fun _a -> h_exists #(U.raise_t a) (U.lift_dom p))
+  : action #immut_heap #no_allocs (h_exists p) unit
+           (fun _a -> h_exists #(FStar.Universe.raise_t a) (FStar.Universe.lift_dom p))
 
 val elim_pure (p:prop)
-  : action (pure p) (u:unit{p}) (fun _ -> emp)
+  : action #immut_heap #no_allocs (pure p) (u:unit{p}) (fun _ -> emp)
 
 val intro_pure (p:prop) (_:squash p)
-  : action emp unit (fun _ -> pure p)
+  : action #immut_heap #no_allocs emp unit (fun _ -> pure p)
 
 val pts_to_evolve (#a:Type u#a) (#pcm:_) (r:ref a pcm) (x y : a) (h:heap)
   : Lemma (requires (interp (pts_to r x) h /\ compatible pcm y x))
           (ensures  (interp (pts_to r y) h))
 
 val drop (p:slprop)
-  : action p unit (fun _ -> emp)
+  : action #immut_heap #no_allocs p unit (fun _ -> emp)
