pulse/lib/pulse/core/PulseCore.Heap2.fst
@@ -256,12 +256,13 @@ let sel_v (#a:Type u#h) (#pcm:pcm a) (r:ref a pcm) (v:erased a) (m:full_hheap (p
   = H.sel_v #a #pcm r v m.concrete
 
 let sel_lemma #a #pcm r m = lower_ptr r m; H.sel_lemma #a #pcm r m.concrete
-let elim_heap_evolves (h0 h1:full_heap)
+let heap_evolves_iff (h0 h1:full_heap)
 : Lemma 
-  (requires heap_evolves h0 h1)
-  (ensures H.heap_evolves h0.concrete h1.concrete /\
-           H.heap_evolves h0.ghost h1.ghost)
-= assert (heap_evolves h0 h1 ==> 
+  (ensures
+     heap_evolves h0 h1 <==> (
+      H.heap_evolves h0.concrete h1.concrete /\
+      H.heap_evolves h0.ghost h1.ghost))
+= assert (heap_evolves h0 h1 <==> 
             (H.heap_evolves h0.concrete h1.concrete /\ H.heap_evolves h0.ghost h1.ghost))
       by (FStar.Tactics.norm [delta_only [`%heap_evolves]])
 
@@ -280,7 +281,7 @@ let witnessed_ref_stability #a #pcm r fact =
       lower_ptr r h0;
       assert (H.interp (H.ptr #a #pcm r) h0.concrete);
       assert (heap_evolves h0 h1);
-      elim_heap_evolves h0 h1;
+      heap_evolves_iff h0 h1;
       assert (H.heap_evolves h0.concrete h1.concrete);
       assert (H.witnessed_ref #a #pcm r fact h1.concrete);
       raise_ptr r h1;
@@ -299,6 +300,7 @@ let lift_heap_pre_action
 
 #restart-solver
 
+#push-options "--fuel 0 --ifuel 0 --z3rlimit_factor 4"
 let lift_action
       (#fp:H.slprop) (#a:Type) (#fp':a -> H.slprop)
       (act:H.action fp a fp')
@@ -346,18 +348,72 @@ let lift_action
       let h00 : H.full_hheap (fp `H.star` hframe) = h0.concrete in
       let h11 : H.full_hheap (fp' x `H.star` hframe) = dsnd (act h00) in
       assert (h1 == { h0 with concrete = h11 });
-      // assr
-      // assert (H.interp (fp' x `H.star` hframe) h1'.concrete);
-      admit()
-    );
-    admit()
-     
-    // let (| x, h1 |) = p h0 in
-    // assert (h1.concrete == dsnd <| act h0.concrete);
-    // assert (H.heap_evolves h0.concrete h1.concrete);
-    // admit();
-    // assert (action_related_heaps frame h0 h1);
-    // admit()
+      H.elim_star (fp' x) hframe h11;
+      eliminate exists c0 c1.
+        H.disjoint c0 c1 /\
+        h11 == H.join c0 c1 /\
+        H.interp (fp' x) c0 /\
+        H.interp hframe c1
+      returns interp (lift (fp' x) `star` frame) h1
+      with _ . ( 
+        let h10 = { concrete = c0; ghost = h0'.ghost } in
+        let h11 = { concrete = c1; ghost = h1'.ghost } in
+        assert (interp (lift (fp' x)) h10);
+        assert (interp frame h11);
+        assert (disjoint h10 h11)
+      );
+      heap_evolves_iff h0 h1;
+      assert (action_related_heaps frame h0 h1)
+    )
   );
   p
- 
+
+let lift_star (p q:H.slprop)
+: Lemma (lift (p `H.star` q) == (lift p `star` lift q))
+        [SMTPat (lift (p `H.star` q))]
+= introduce forall m.
+    interp (lift (p `H.star` q)) m <==>
+    interp (lift p `star` lift q) m
+  with (
+    introduce 
+      interp (lift p `star` lift q) m ==>
+      interp (lift (p `H.star` q)) m
+    with _ . ( 
+      eliminate exists h0 h1.
+        disjoint h0 h1 /\
+        m == join h0 h1 /\
+        interp (lift p) h0 /\
+        interp (lift q) h1
+      returns interp (lift (p `H.star` q)) m
+      with _ . (
+        H.intro_star p q h0.concrete h1.concrete
+      )
+    );
+    introduce 
+      interp (lift (p `H.star` q)) m ==>
+      interp (lift p `star` lift q) m
+    with _ . ( 
+      H.elim_star p q m.concrete;
+      eliminate exists c0 c1.
+        H.disjoint c0 c1 /\
+        m.concrete == H.join c0 c1 /\
+        H.interp p c0 /\
+        H.interp q c1
+      returns interp (lift p `star` lift q) m
+      with _ . (
+        let h0 = { concrete = c0; ghost = m.ghost } in
+        let h1 = { concrete = c1; ghost = H.empty_heap } in
+        assert (disjoint h0 h1)
+      )
+    )
+  );
+  slprop_extensionality (lift (p `H.star` q)) (lift p `star` lift q)
+
+let sel_action #a #pcm r v0 = lift_action (H.sel_action #a #pcm r v0)
+let select_refine #a #p r x f = lift_action (H.select_refine #a #p r x f)
+let upd_gen_action #a #p r x y f = lift_action (H.upd_gen_action #a #p r x y f)
+let upd_action #a #p r x y = lift_action (H.upd_action #a #p r x y)
+let free_action #a #p r v0 = lift_action (H.free_action #a #p r v0)
+let split_action #a #p r v0 v1 = lift_action (H.split_action #a #p r v0 v1)
+let gather_action #a #p r v0 v1 = lift_action (H.gather_action #a #p r v0 v1)
+let pts_to_not_null_action #a #p r v = lift_action (H.pts_to_not_null_action #a #p r v)
